add extraction the encoding function to C

code/experimental/rsa/RSA.fst
@@ -5,8 +5,7 @@ open FStar.ST
 open FStar.Buffer
 open FStar.Int.Cast
 open FStar.All
-
-open BN.Convert
+open FStar.Mul
 
 module U32 = FStar.UInt32
 module U8 = FStar.UInt8
@@ -14,243 +13,179 @@ module U8 = FStar.UInt8
 type uint8_p = buffer FStar.UInt8.t
 type bignum = buffer FStar.UInt64.t
 
-type rsa_pubkey = (n:bignum * e:bignum)
-type rsa_privkey = (rsa_pubkey * d:bignum)
+type rsa_pubkey = 
+	| Mk_rsa_pubkey: n:bignum -> e:bignum -> rsa_pubkey
+
+type rsa_privkey =
+	| Mk_rsa_privkey: pkey:rsa_pubkey -> d:bignum -> rsa_privkey
 
 let zero_8 = 0uy
-let zero_64 = 0uL
-let hash_size_sha256 = 32ul
-let bn_bytes = 8ul
+let hLen = 32ul
+let sLen = 20ul
 
-assume val hash_sha256: m: uint8_p -> mHash: uint8_p {length mHash = 32} -> ST unit 
+assume val nat_to_text: n:bignum -> len:U32.t -> res:uint8_p{length res = U32.v len} -> ST unit
+(requires (fun h -> live h n /\ live h res))
+(ensures (fun h0 _ h1 -> live h0 n /\ live h0 res /\ live h1 res /\ modifies_1 res h0 h1))
+
+assume val text_to_nat: text:uint8_p -> res:bignum -> ST unit 
+(requires (fun h -> live h text /\ live h res))
+(ensures (fun h0 _ h1 -> live h0 text /\ live h0 res /\ live h1 res /\ modifies_1 res h0 h1))
+
+val get_octets: modBits:U32.t -> Tot U32.t
+let get_octets modBits = U32.((modBits +^ 7ul) /^ 8ul)
+
+val get_length_em: modBits:U32.t -> Tot U32.t
+let get_length_em modBits =
+	let k = get_octets modBits in
+	if U32.((modBits -^ 1ul) %^ 8ul =^ 0ul) 
+	then U32.(k -^ 1ul) else k
+
+val hash_sha256: mHash:uint8_p{length mHash = 32} -> m:uint8_p -> len:U32.t{U32.v len = length m} -> ST unit 
 (requires (fun h -> live h m /\ live h mHash))
-(ensures (fun h0 _ h1 -> live h0 m /\ live h0 mHash /\ live h1 m /\ live h1 mHash /\ modifies_1 mHash h0 h1))
+(ensures (fun h0 _ h1 -> live h0 m /\ live h0 mHash /\ live h1 mHash /\ modifies_1 mHash h0 h1))
+let hash_sha256 mHash m len = SHA2_256.hash mHash m len
 
-assume val random_bytes: sLen:U32.t -> s:uint8_p {length s = U32.v sLen} -> ST unit
-(requires (fun h -> live h s))
-(ensures (fun h0 _ h1 -> live h0 s /\ live h1 s /\ modifies_1 s h0 h1))
-
-val get_octets: (num_bits: U32.t) -> Tot U32.t
-let get_octets num_bits = U32.((num_bits +^ 7ul) /^ 8ul)
-
-val maskeddb:
-salt: uint8_p ->
-em: uint8_p ->
-sLen: U32.t {U32.v sLen <= length salt /\ U32.v sLen <= length em} ->
-i: U32.t {U32.v i + U32.v sLen <= length em} -> ST unit
-(requires (fun h -> live h salt /\ live h em))
-(ensures (fun h0 _ h1 -> live h0 salt /\ live h0 em /\ live h1 salt /\ live h1 em /\  modifies_1 em h0 h1))
-let rec maskeddb salt em sLen i =
-	if U32.(sLen >^ 0ul)
-	then (let sLen = U32.(sLen -^ 1ul) in
-		 let em_i = U32.(i +^ sLen) in
-		 em.(em_i) <- U8.(em.(em_i) ^^ salt.(sLen));
-		 maskeddb salt em sLen i)
-	else ()
-
-val mgf1: res: uint8_p -> len: U32.t -> seed: uint8_p -> seed_len: U32.t -> i: U32.t -> ST unit
-(requires (fun h -> live h res /\ live h seed))
-(ensures (fun h0 _ h1 -> live h1 res /\ live h1 seed /\  modifies_1 res h0 h1))
-let rec mgf1 res len seed seed_len i =
-	let mdLen = hash_size_sha256 in
-	if U32.(len >^ 0ul)
-	then
-		let counter = create zero_8 4ul in
-		counter.(0ul) <- uint32_to_uint8 (U32.(i >>^ 24ul));
-		counter.(1ul) <- uint32_to_uint8 (U32.(i >>^ 16ul));
-		counter.(2ul) <- uint32_to_uint8 (U32.(i >>^ 8ul));
-		counter.(3ul) <- uint32_to_uint8 i;
-		let ctx = create zero_8 U32.(seed_len +^ 4ul) in
-		blit seed 0ul ctx 0ul seed_len;
-		blit counter 0ul ctx seed_len 4ul;
-		let hash_ctx = create zero_8 hash_size_sha256 in
-		hash_sha256 ctx hash_ctx;
-		if U32.(mdLen <=^ len)
-		then (blit hash_ctx 0ul res U32.(i *^ mdLen) mdLen;
-			 mgf1 res U32.(len -^ mdLen) seed seed_len U32.(i +^ 1ul))
-		else blit hash_ctx 0ul res U32.(i *^ mdLen) len
+val mgf: mgfseed_len:U32.t -> mgfseed:uint8_p{length mgfseed = U32.v mgfseed_len} ->  
+	len:U32.t -> counter:U32.t -> acc:uint8_p{length acc = U32.(v (hLen *^ counter))} -> 
+	res:uint8_p{length res = U32.v len} -> ST unit
+	(requires (fun h -> live h res /\ live h mgfseed /\ live h acc))
+	(ensures (fun h0 _ h1 -> live h0 res /\ live h0 mgfseed /\ live h0 acc /\ live h1 res /\ modifies_1 res h0 h1)) 
+let rec mgf mgfseed_len mgfseed len counter acc res =
+	(* if len > op_Multiply (pow2 32) hLen then failwith "mask too long" *)
+	push_frame();
+	let c = create zero_8 4ul in
+	c.(0ul) <- uint32_to_uint8 (U32.(counter >>^ 24ul));
+	c.(1ul) <- uint32_to_uint8 (U32.(counter >>^ 16ul));
+	c.(2ul) <- uint32_to_uint8 (U32.(counter >>^ 8ul));
+	c.(3ul) <- uint32_to_uint8 counter;
+	let tmp = create zero_8 U32.(mgfseed_len +^ 4ul) in
+	blit mgfseed 0ul tmp 0ul mgfseed_len;
+	blit c 0ul tmp mgfseed_len 4ul;
+	let hash_tmp = create zero_8 hLen in
+	hash_sha256 hash_tmp tmp U32.(mgfseed_len +^ 4ul);
+	let counter = U32.(counter +^ 1ul) in
+	let acc_size = U32.(counter *^ hLen) in
+	let acc_tmp = create zero_8 acc_size in
+	blit acc 0ul acc_tmp 0ul U32.(acc_size -^ hLen);
+	blit hash_tmp 0ul acc_tmp U32.(acc_size -^ hLen) hLen;
+	if U32.(acc_size <^ len)
+	then mgf mgfseed_len mgfseed len counter acc_tmp res
+	else blit acc_tmp 0ul res 0ul len;
+	pop_frame()
 
 val xordb:
-db: uint8_p -> 
-len: U32.t {U32.v len <= length db} -> 
-em: uint8_p -> 
-i: U32.t {U32.v i + U32.v len <= length db /\ U32.v i + U32.v len <= length em} -> ST unit
-(requires (fun h -> live h db /\ live h em))
-(ensures (fun h0 _ h1 -> live h0 db /\ live h0 em /\ live h1 db /\ live h1 em /\  modifies_1 db h0 h1))
-let rec xordb db len em i =
-	if U32.(len >^ 0ul)
-	then
+	b1:uint8_p ->
+	b2:uint8_p{length b2 = length b1} -> 
+	len:U32.t{U32.v len <= length b1} -> ST unit
+	(requires (fun h -> live h b1 /\ live h b2))
+	(ensures (fun h0 _ h1 -> live h0 b1 /\ live h0 b2 /\ live h1 b1 /\ modifies_1 b1 h0 h1))
+	(decreases len)
+let rec xordb b1 b2 len =
+	push_frame();
+	if U32.(len >^ 0ul) then
 		let len = U32.(len -^ 1ul) in
-		let db_i = U32.(i +^ len) in
-		db.(db_i) <- U8.(db.(db_i) ^^ em.(db_i));
-		xordb db len em i
-	else ()
+		b1.(len) <- U8.(b1.(len) ^^ b2.(len));
+		xordb b1 b2 len
+	else ();
+	pop_frame()
 
-val get_index_01: db: uint8_p -> len: U32.t -> i: U32.t -> ST U32.t
-(requires (fun h -> live h db))
-(ensures (fun h0 _ h1 -> live h1 db /\ h1 == h0))
-let rec get_index_01 db len i =
-	if U32.(len >^ 0ul)
-	then if U8.(db.(i) =^ zero_8)
-		 then get_index_01 db U32.(len -^ 1ul) U32.(i +^ 1ul)
-		 else i
-	else i
-
-val rsa_padding_add_PKSC1_PSS_mgf1: num_bits: U32.t -> skey: rsa_privkey -> em: uint8_p -> mHash: uint8_p -> ST unit
-(requires (fun h -> live h em /\ live h mHash)) (* live h skey *)
-(ensures (fun h0 _ h1 -> live h1 em /\ live h1 mHash /\  modifies_1 em h0 h1))
-let rsa_padding_add_PKSC1_PSS_mgf1 num_bits skey em mHash =
-	(* if n = 0 then error *)
-	let hLen = hash_size_sha256 in
-	let msBits = U32.((num_bits -^ 1ul) &^ 7ul) in
-	let emLen = get_octets num_bits in
-	let emLen = if U32.(msBits =^ 0ul) then U32.(emLen -^ 1ul) else emLen in
-	let em = if U32.(msBits =^ 0ul) then offset em 1ul else em in
-	(* if U32.(emLen <^ hLen +^ 2ul) then failwith "message too long"; *)
-	let sLen = U32.(emLen -^ hLen -^ 2ul) in
-	let salt = create zero_8 sLen in
-	if U32.(sLen >^ 0ul) then random_bytes sLen salt;
-	
-	let size_m1 = U32.(8ul +^ hLen +^ sLen) in
-	let m1 = create zero_8 size_m1 in
+val pss_encode: 
+	modBits:U32.t{U32.v (get_length_em modBits) >= U32.(v (sLen +^ hLen +^ 2ul))} ->
+	msg:uint8_p -> len:U32.t{U32.v len = length msg} ->
+	salt:uint8_p{length salt = U32.v sLen} ->
+	em:uint8_p{length em = U32.v (get_length_em modBits)} -> ST unit
+	(requires (fun h -> live h msg /\ live h em /\ live h salt))
+	(ensures (fun h0 _ h1 -> live h0 msg /\ live h0 em /\  live h0 salt /\ live h1 salt /\ live h1 em /\ modifies_1 em h0 h1))
+let pss_encode modBits msg len salt em =
+	push_frame();
+	let mHash = create zero_8 hLen in
+	hash_sha256 mHash msg len;
+	let emBits = U32.(modBits -^ 1ul) in
+	let emLen = get_length_em modBits in
+	let m1_size = U32.(8ul +^ hLen +^ sLen) in
+	let m1 = create zero_8 m1_size in
 	(* first 8 elements should be 0x00 *)
 	blit mHash 0ul m1 8ul hLen;
-	if U32.(sLen >^ 0ul)
-	then blit salt 0ul m1 U32.(8ul +^ hLen) sLen;
-	let hash_m1 = create zero_8 hash_size_sha256 in
-	hash_sha256 m1 hash_m1;
+	blit salt 0ul m1 U32.(8ul +^ hLen) sLen;
+	let m1Hash = create zero_8 hLen in
+	hash_sha256 m1Hash m1 m1_size;
 	
-	let maskedDBLen = U32.(emLen -^ hLen -^ 1ul) in
-	blit hash_m1 0ul em maskedDBLen hLen;
-	mgf1 em maskedDBLen hash_m1 hLen 0ul;
+	let db_size = U32.(emLen -^ hLen -^ 1ul) in
+	let db = create zero_8 db_size in
+	let ind_1 = U32.(emLen -^ sLen -^ hLen -^ 2ul) in
+	db.(ind_1) <- 1uy;
+	blit salt 0ul db U32.(ind_1 +^ 1ul) sLen;
+	
+	let dbMask = create zero_8 db_size in
+	let acc = create zero_8 0ul in
+	mgf hLen m1Hash db_size 0ul acc dbMask;
 
-	let i1 = U32.(emLen -^ sLen -^ hLen -^ 2ul) in
-	em.(i1) <- U8.(em.(i1) ^^ 1uy);
-	if U32.(sLen >^ 0ul) then maskeddb salt em sLen U32.(i1 +^ 1ul);
+	xordb db dbMask db_size;
+	let zeroL = U32.(8ul *^ emLen -^ emBits) in
+	db.(0ul) <- U8.(db.(0ul) &^ (0xffuy >>^ zeroL));
 
-	if U32.(msBits >^ 0ul)
-	then em.(0ul) <- U8.(em.(0ul) &^ (0xffuy >>^ U32.(8ul -^ msBits)));
-	
-	upd em U32.(emLen -^ 1ul) 0xbcuy
+	blit db 0ul em 0ul db_size;
+	blit m1Hash 0ul em db_size hLen;
+	upd em U32.(emLen -^ 1ul) 0xbcuy;
+	pop_frame()
 
-assume val rsa_sign_raw: num_bits:U32.t -> skey: rsa_privkey -> em: uint8_p -> result: uint8_p -> ST unit
-(requires (fun h -> live h em /\ live h result)) (* live h skey *)
-(ensures (fun h0 _ h1 -> live h1 em /\ live h1 result /\  modifies_1 result h0 h1))
-(*
-let rsa_sign_raw num_bits skey em result =
-	(* not (is_zero mod) *)
-	(* is_odd mod *)
-	(* not (is_negative mod) *)
-	let n = fst (fst skey) in
-	let e = fst (snd skey) in
-	let d = snd skey in
-	let len = get_octets num_bits in
-	
-	let f_size = U32.((len -^ 1ul) /^ bn_bytes +^ 1ul) in
-	let f = create zero_64 f_size in
-	bn_bin2bn em len f;
-	
-	let n0 = bn_mont_n0 n in
-	let lgBigR = U32.(num_bits +^ (bn_bits2 -^ 1ul)) /^ bn_bits2 *^ bn_bits2 in
-	let rr = create zero_64 len in
-	bn_mod_exp_base_2 num_bits rr (U32.(lgBigR *^ 2)) n;
-	let mont = Mk_mont_n n rr n0 in
-	
-	let b_a = create zero_64 len in
-	let b_ai = create zero_64 len in
-	let b = Mk_blinding_t b_a b_ai in
-	
-	bn_blinding_create_param b e mont;
-	bn_mod_mul_montgomery f b_a mont;
-	let result = create zero_64 len in
-	bn_mod_exp_mont_consttime result f d n mont;
-	
-	(* VERIFY the result to protect against fault attacks
-	let vrfy = create zero_64 len in
-	bn_mod_exp_mont vrfy result e n mont_n;
-	if not (eqb vrfy result) then failwith "error" *)
-	
-	bn_blinding_invert result b mont;
-	
-	bn_bn2bin_padded len out result
-*)
+val pss_verify:
+	modBits:U32.t{U32.v (get_length_em modBits) >= U32.(v (sLen +^ hLen +^ 2ul))} ->
+	em:uint8_p{length em = U32.v (get_length_em modBits)} ->
+	msg:uint8_p -> len:U32.t{U32.v len = length msg} -> ST bool
+	(requires (fun h -> live h msg /\ live h em))
+	(ensures (fun h0 _ h1 -> live h0 msg /\ live h0 em /\ live h1 msg /\ live h1 em))
+let pss_verify modBits em msg len =
+	push_frame();
+	let mHash = create zero_8 hLen in
+	hash_sha256 mHash msg len;
+	let emLen = get_length_em modBits in
+	let res = 
+	if not (U8.(em.(U32.(emLen -^ 1ul)) =^ 0xbcuy)) then false else (
+	let db_size = U32.(emLen -^ hLen -^ 1ul) in
+	let maskedDB = sub em 0ul db_size in
+	let m1Hash = sub em db_size hLen in
+	let zeroL = U32.(8ul *^ emLen -^ (modBits -^ 1ul)) in
+	let tmp = U8.(maskedDB.(0ul) &^ (0xffuy <<^ U32.(8ul -^ zeroL))) in
+	if not (U8.(tmp =^ 0x00uy)) then false else (
+	let dbMask = create zero_8 db_size in
+	let acc = create zero_8 0ul in
+	mgf hLen m1Hash db_size 0ul acc dbMask;
+	xordb maskedDB dbMask db_size;
+	maskedDB.(0ul) <- U8.(maskedDB.(0ul) &^ (0xffuy >>^ zeroL));
 
-val rsa_sha256_sign: num_bits:U32.t -> result: uint8_p{length result = U32.v (get_octets num_bits)} -> skey: rsa_privkey -> msg: uint8_p -> ST unit
-(requires (fun h -> live h result /\ live h msg))  (* live h skey *)
-(ensures (fun h0 _ h1 -> live h1 result /\ live h1 msg /\  modifies_1 result h0 h1))
-let rsa_sha256_sign num_bits result skey msg =
-	let mHash = create zero_8 hash_size_sha256 in
-	hash_sha256 msg mHash;
-	let size = get_octets num_bits in
-	let em = create zero_8 size in
-	rsa_padding_add_PKSC1_PSS_mgf1 num_bits skey em mHash; (* mHash -> em, |em| = k \/ |em| = k - 1 *)
-	rsa_sign_raw num_bits skey em result (* |result| = k *)
+	let pad_size = U32.(emLen -^ sLen -^ hLen -^ 1ul) in
+	let pad2 = create zero_8 pad_size in
+	upd pad2 U32.(pad_size -^ 1ul) 0x01uy;
 
-assume val rsa_verify_raw: num_bits:U32.t -> pkey: rsa_pubkey -> sig: uint8_p -> em: uint8_p -> ST unit
-(requires (fun h -> live h sig /\ live h em))
-(ensures (fun h0 _ h1 -> live h1 sig /\ live h1 em))
-(*
-let rsa_verify_raw num_bits pkey sig em = 
-	let len = get_octets num_bits in
-	let n = fst pkey in
-	let e = snd pkey in
-	
-	(* let cond = check_modulus_and_exponent_sizes n in *)
-	
-	let f_size = U32.((len -^ 1ul) /^ bn_bytes +^ 1ul) in
-	let f = create zero_64 f_size in
-	bn_bin2bn sig len f;
-	
-	let n0 = bn_mont_n0 n in
-	let lgBigR = U32.(num_bits +^ (bn_bits2 -^ 1ul)) /^ bn_bits2 *^ bn_bits2 in
-	let rr = create zero_64 len in
-	bn_mod_exp_base_2 num_bits rr (U32.(lgBigR *^ 2)) n;
-	let mont = Mk_mont_n n rr n0 in
-	
-	let result = create zero_64 len in
-	bn_mod_exp_mont result f e n mont;
-	
-	bn_bn2bin_padded len em result
-*)
+	let pad = sub maskedDB 0ul pad_size in
+	if not (eqb pad pad2 pad_size) then false else (
+	let salt = sub maskedDB pad_size sLen in
+	let m1_size = U32.(8ul +^ hLen +^ sLen) in
+	let m1 = create zero_8 m1_size in
+	(* first 8 elements should be 0x00 *)
+	blit mHash 0ul m1 8ul hLen;
+	blit salt 0ul m1 U32.(8ul +^ hLen) sLen;
+	let m1Hash' = create zero_8 hLen in
+	hash_sha256 m1Hash' m1 m1_size;
+	eqb m1Hash m1Hash' hLen
+	))) in
+	pop_frame();
+	res
 
-val rsa_verify_PKCS1_PSS_mgf1: num_bits:U32.t -> pkey: rsa_pubkey -> em: uint8_p -> mHash: uint8_p -> ST bool
-(requires (fun h -> live h em /\ live h mHash))
-(ensures (fun h0 _ h1 -> live h1 em /\ live h1 mHash))
-let rsa_verify_PKCS1_PSS_mgf1 num_bits pkey em mHash =
-	let hLen = hash_size_sha256 in
-	let msBits = U32.((num_bits -^ 1ul) &^ 7ul) in
-	let emLen = get_octets num_bits in
-	if U8.((em.(0ul) &^ (0xffuy <<^ msBits)) >^ 0uy) then false else
-	let emLen = if U32.(msBits =^ 0ul) then U32.(emLen -^ 1ul) else emLen in
-	let em = if U32.(msBits =^ 0ul) then offset em 1ul else em in
-	(* error if emLen < hLen *)
-	let i = U32.(emLen -^ 1ul) in
-	if not (U8.(em.(i) =^ 0xbcuy)) then false else
-	let maskedDBLen = U32.(emLen -^ hLen -^ 1ul) in
-	let h = sub em maskedDBLen hLen in
-	let db = create zero_8 maskedDBLen in
-	mgf1 db maskedDBLen h hLen 0ul;
-	xordb db maskedDBLen em 0ul;
-	if U32.(msBits >^0ul) then db.(0ul) <- U8.(db.(0ul) &^ (0xffuy >>^ U32.(8ul -^ msBits)));
-	let i = get_index_01 db maskedDBLen 0ul in (* i <= maskedDBLen *)
-	if not (U8.(db.(i) =^ 1uy)) then false else 
-	let sLen = U32.(maskedDBLen -^ i) in
-	let salt = sub db sLen U32.(i +^ 1ul) in
-	let h_size = U32.(8ul +^ hLen +^ sLen) in
-	let h_ = create zero_8 h_size in
-	blit mHash 0ul h_ 8ul hLen;
-	if U32.(sLen >^ 0ul) then blit salt 0ul h_ U32.(8ul +^ hLen) sLen;
-	let h_hash = create zero_8 hash_size_sha256 in
-	hash_sha256 h_ h_hash;
-	eqb h_hash h hLen
+assume val rsa_sign:
+	modBits:U32.t{U32.v (get_length_em modBits) >= U32.(v (sLen +^ hLen +^ 2ul))} ->
+	msg:uint8_p ->
+	skey:rsa_privkey -> 
+	salt:uint8_p{length salt = U32.v sLen} ->
+	sgnt:uint8_p{length sgnt = U32.v (get_octets modBits)} -> ST unit
+	(requires (fun h -> live h msg /\ live h salt))
+	(ensures (fun h0 _ h1 -> live h0 msg /\ live h0 salt /\ live h1 msg /\ live h1 salt))
 
-val rsa_sha256_verify: num_bits:U32.t -> sig: uint8_p {length sig = U32.v (get_octets num_bits)} -> pkey: rsa_pubkey -> msg: uint8_p -> ST bool
-(requires (fun h -> live h sig /\ live h msg))
-(ensures (fun h0 _ h1 -> live h1 sig /\ live h1 msg))
-let rsa_sha256_verify num_bits sig pkey msg =
-	let size = get_octets num_bits in
-	let em = create zero_8 size in
-	rsa_verify_raw num_bits pkey sig em;
-	let mHash = create zero_8 hash_size_sha256 in
-	hash_sha256 msg mHash;
-	rsa_verify_PKCS1_PSS_mgf1 num_bits pkey em mHash
+assume val rsa_verify:
+	modBits:U32.t{U32.v (get_length_em modBits) >= U32.(v (sLen +^ hLen +^ 2ul))} ->
+	sgnt:uint8_p{length sgnt = U32.v (get_octets modBits)} ->
+	pkey:rsa_pubkey -> 
+	msg:uint8_p -> ST bool
+	(requires (fun h -> live h msg /\ live h sgnt))
+	(ensures (fun h0 _ h1 -> live h0 msg /\ live h0 sgnt /\ live h1 msg /\ live h1 sgnt))
